Change external choice semantics, compile choice before payloads
Greatly simplifies payloadLang + makes semantics reflection hold
even for endpointLang processes that are not in the range of
endpoint projection.

The problem previously was that

  NEndpoint p1 s1 (Send p2 [2w])
  | NEndpoint p2 s2 (ExtChoice p1 e1 e2)

has no transitions in p2, whereas the resulting process after choice
elimination:

  NEndpoint p1 s1 (Send p2 [2w])
  | NEndpoint p2 s2 (Receive p1 fv (IfThen fv e1 e2))

p2 can reduce to e2.

This commit endeavours to repair this discrepancy by bringing choice semantics
closer to ifthenelse semantics.

projection/endpointSemanticsScript.sml
@@ -92,8 +92,9 @@ val (trans_rules,trans_ind,trans_cases) = Hol_reln `
              (NEndpoint p2 (s with queue := q1 ++ q2) e1))
 
   (* ExtChoice-R *)
-∧ (∀s p1 p2 e1 e2 q1 q2.
-    s.queue = q1 ++ [(p1,[0w])] ++ q2
+∧ (∀s p1 p2 e1 e2 q1 d q2.
+    s.queue = q1 ++ [(p1,d)] ++ q2
+    ∧ d ≠ [1w]
     ∧ p1 ≠ p2
     ∧ EVERY (λ(p,_). p ≠ p1) q1 
     ⇒ trans (NEndpoint p2 s (ExtChoice p1 e1 e2))
@@ -137,12 +138,20 @@ val (trans_rules,trans_ind,trans_cases) = Hol_reln `
 `
 
 val _ = zip ["trans_send","trans_enqueue","trans_com_l","trans_com_r","trans_int_choice",
-              "enqueue_choice_l","enqueue_choice_r","com_choice_l","com_choice_r",
+              "trans_enqueue_choice_l","trans_enqueue_choice_r","trans_com_choice_l","trans_com_choice_r",
               "trans_dequeue","trans_ext_choice_l","trans_ext_choice_r",
               "trans_if_true","trans_if_false","trans_let","trans_par_l","trans_par_r"]
             (CONJUNCTS trans_rules) |> map save_thm;
 
 val reduction_def = Define `
   reduction p q = trans p LTau q`
+
+val weak_tau_trans_def = Define `
+  weak_tau_trans p alpha q =
+    ?p' q'. reduction^* p p' /\ trans p' alpha q' /\ reduction^* q' q`
+
+val weak_trans_def = Define `
+  weak_trans p alpha q =
+    if alpha = LTau then reduction^* p q else weak_tau_trans p alpha q`
 
 val _ = export_theory ()
