projection/payloadSemanticsScript.sml
@@ -5,8 +5,6 @@ val _ = new_theory "payloadSemantics";
 val _ = Datatype `
  label = LSend proc datum proc
        | LReceive proc datum proc
-       | LIntChoice proc bool proc
-       | LExtChoice proc bool proc
        | LTau
 `
 
@@ -49,39 +47,6 @@ val (trans_rules,trans_ind,trans_cases) = Hol_reln `
     ∧ trans conf n2 (LSend p1 d p2) n2'
     ⇒ trans conf (NPar n1 n2) LTau (NPar n1' n2'))
 
-  (* IntChoice *)
-∧ (∀conf s b p1 p2 e.
-    p1 ≠ p2
-    ⇒ trans conf (NEndpoint p1 s (IntChoice b p2 e)) (LIntChoice p1 b p2) (NEndpoint p1 s e))
-
-  (* Enqueue-Choice-L *)
-∧ (∀conf s p1 p2 e.
-    p1 ≠ p2
-    ⇒ trans conf (NEndpoint p2 s e)
-             (LExtChoice p1 T p2)
-             (NEndpoint p2 (s with queue := SNOC (p1,[6w;1w]) s.queue) e))
-
-  (* Enqueue-Choice-R *)
-∧ (∀conf s p1 p2 e.
-    p1 ≠ p2
-    ⇒ trans conf (NEndpoint p2 s e)
-             (LExtChoice p1 F p2)
-             (NEndpoint p2 (s with queue := SNOC (p1,[6w;0w]) s.queue) e))
-
-  (* Com-Choice-L *)
-∧ (∀conf n1 n2 p1 p2 b n1' n2'.
-    p1 ≠ p2
-    ∧ trans conf n1 (LIntChoice p1 b p2) n1'
-    ∧ trans conf n2 (LExtChoice p1 b p2) n2'
-    ⇒ trans conf (NPar n1 n2) LTau (NPar n1' n2'))
-
-  (* Com-Choice-R *)
-∧ (∀conf n1 n2 p1 p2 d n1' n2'.
-    p1 ≠ p2
-    ∧ trans conf n1 (LExtChoice p1 d p2) n1'
-    ∧ trans conf n2 (LIntChoice p1 d p2) n2'
-    ⇒ trans conf (NPar n1 n2) LTau (NPar n1' n2'))
-
   (* Dequeue-last-payload *)
 ∧ (∀conf s v p1 p2 e q1 q2 d ds.
     s.queue = q1 ++ [(p1,6w::d)] ++ q2
@@ -100,24 +65,6 @@ val (trans_rules,trans_ind,trans_cases) = Hol_reln `
     ⇒ trans conf (NEndpoint p2 s (Receive p1 v ds e))
              LTau
              (NEndpoint p2 (s with queue := q1 ++ q2) (Receive p1 v (SNOC d ds) e)))
-
-  (* ExtChoice-L *)
-∧ (∀conf s p1 p2 e1 e2 q1 q2.
-    s.queue = q1 ++ [(p1,[6w;1w])] ++ q2
-    ∧ p1 ≠ p2
-    ∧ EVERY (λ(p,_). p ≠ p1) q1 
-    ⇒ trans conf (NEndpoint p2 s (ExtChoice p1 e1 e2))
-             LTau
-             (NEndpoint p2 (s with queue := q1 ++ q2) e1))
-
-  (* ExtChoice-R *)
-∧ (∀conf s p1 p2 e1 e2 q1 q2.
-    s.queue = q1 ++ [(p1,[6w;0w])] ++ q2
-    ∧ p1 ≠ p2
-    ∧ EVERY (λ(p,_). p ≠ p1) q1 
-    ⇒ trans conf (NEndpoint p2 s (ExtChoice p1 e1 e2))
-             LTau
-             (NEndpoint p2 (s with queue := q1 ++ q2) e2))
 
   (* If-L *)
 ∧ (∀conf s v p e1 e2.
@@ -156,10 +103,8 @@ val (trans_rules,trans_ind,trans_cases) = Hol_reln `
 `
 
  val _ = zip ["trans_send_last_payload","trans_send_intermediate_payload",
-              "trans_enqueue","trans_com_l","trans_com_r","trans_int_choice",
-              "trans_enqueue_choice_l","trans_enqueue_choice_r","trans_com_choice_l","trans_com_choice_r",
+              "trans_enqueue","trans_com_l","trans_com_r",
               "trans_dequeue_last_payload","trans_dequeue_intermediate_payload",
-              "trans_ext_choice_l","trans_ext_choice_r",
               "trans_if_true","trans_if_false","trans_let","trans_par_l","trans_par_r"]
             (CONJUNCTS trans_rules) |> map save_thm;
 
